finished up lemmas for host liftings, renamed some lemmas

theories/iris_host.v
@@ -1,11 +1,14 @@
 From mathcomp Require Import ssreflect eqtype seq ssrbool ssrfun.
-From iris.program_logic Require Import language.
+From iris.program_logic Require Import language weakestpre lifting.
 From iris.proofmode Require Import base tactics classes.
 From iris.base_logic Require Export gen_heap ghost_map proph_map.
 From iris.base_logic.lib Require Export fancy_updates.
 (* From iris.bi Require Export weakestpre. *)
-Require Export iris iris_locations iris_properties iris_wp stdpp_aux.
+Require Export iris_locations iris_properties stdpp_aux iris.
 Require Export datatypes host operations properties opsem instantiation.
+
+
+
 
 Section Iris_host.
 
@@ -34,16 +37,11 @@ Definition vimp : Type := vi * (seq.seq Byte.byte).
 Inductive inst_decl: Type :=
   ID_instantiate: vi -> nat -> list vimp -> inst_decl.
 
-Definition host_prog : Type := (list module) * (list inst_decl).
-
-Definition host_config : Type := store_record * vi_store * host_prog * (list administrative_instruction).
+Definition host_config : Type := store_record * vi_store * (list module) * (list inst_decl) * (list administrative_instruction).
 
 Definition instantiate := instantiate host_function host_instance.
 
-Print module_export.
-
-Print name.
-
+(* Does the start function always take 0 arguments? *)
 Definition map_start (start: option nat) : list administrative_instruction :=
   match start with
   | Some n => [AI_invoke n]
@@ -67,6 +65,9 @@ Definition lookup_export_vi (vis: vi_store) (vimp: vimp) : option module_export_
 Definition empty_instance := Build_instance [::] [::] [::] [::] [::].
 Definition empty_frame := Build_frame [::] empty_instance.
 
+(* Dummy *)
+Parameter hs: host_state host_instance.
+
 Inductive host_reduce: host_config -> host_config -> Prop :=
 | HR_host_step: forall s vis m vi vm vimps imps s' vis' ms idecs' inst exps start vs,
     ms !! vm = Some m ->
@@ -74,9 +75,392 @@ Inductive host_reduce: host_config -> host_config -> Prop :=
     instantiate s m imps ((s', inst, exps), start) ->
     const_list vs ->
     vis' = <[ vi := exps ]> vis ->
-    host_reduce (s, vis, (ms, (ID_instantiate vi vm vimps) :: idecs'), vs) (s', vis', (ms, idecs'), map_start start)
-| HR_wasm_step: forall s vis ms idecs s' es es' hs hs',
-    reduce hs s empty_frame es hs' s' empty_frame es' ->
-    host_reduce (s, vis, (ms, idecs), es) (s', vis, (ms, idecs), es').
-    
+    host_reduce (s, vis, ms, (ID_instantiate vi vm vimps) :: idecs', vs) (s', vis', ms, idecs', map_start start)
+| HR_wasm_step: forall s vis ms idecs s' es es' hs',
+    (* No reentrancy and no host functions, so hs should just be dummy *)
+    opsem.reduce hs s empty_frame es hs' s' empty_frame es' ->
+    host_reduce (s, vis, ms, idecs, es) (s', vis, ms, idecs, es').
+
+Definition host_expr : Type := (list inst_decl) * (list administrative_instruction).
+
+(* val is the same as native Wasm, defined in Iris.v *)
+(*
+Definition val_eq_dec : forall v1 v2: val, {v1 = v2} + {v1 <> v2}.
+Proof.
+  decidable_equality.
+Defined.
+Definition val_eqb (v1 v2: val) : bool := val_eq_dec v1 v2.
+Definition eqvalP : Equality.axiom val_eqb :=
+  eq_dec_Equality_axiom val_eq_dec.
+
+Canonical Structure val_eqMixin := EqMixin eqvalP.
+Canonical Structure val_eqType := Eval hnf in EqType val val_eqMixin.
+*)
+
+
+Definition state : Type := store_record * vi_store * (list module) .
+
+Definition observation := unit. 
+
+Definition of_val (v: val) : host_expr := ([::], iris.of_val v).
+
+Lemma of_val_imm (vs : list value) :
+  ([::], ((λ v : value, AI_basic (BI_const v)) <$> vs)) = of_val (immV vs).
+Proof. done. Qed.
+
+Definition to_val (e: host_expr) : option val :=
+  match e with
+  | (e' :: es, _) => None
+  | ([::], wes) => iris.to_val wes
+  end.
+
+Definition prim_step (e : host_expr) (s : state) (os : list observation) (e' : host_expr) (s' : state) (fork_es' : list host_expr) : Prop :=
+  let '(ws, vis, ms) := s in
+  let '(ws', vis', ms') := s' in
+  let '(hes, wes) := e in
+  let '(hes', wes') := e' in
+    host_reduce (ws, vis, ms, hes, wes) (ws', vis', ms', hes', wes') /\ os = [] /\ fork_es' = [].
+
+Lemma to_of_val v : to_val (of_val v) = Some v.
+Proof.
+  destruct 0 => //.
+  move: l.
+  elim => //=.
+  move => v0 v IH.
+  by rewrite IH.
+Qed.
+
+Lemma of_to_val e v : to_val e = Some v → of_val v = e.
+Proof.
+  destruct e as [hes wes] => /=.
+  destruct hes => //.
+  move => Htv; apply iris.of_to_val in Htv.
+  unfold of_val.
+  by f_equal.
+Qed.
+
+Lemma val_head_stuck : forall e1 s1 κ e2 s2 efs,
+  prim_step e1 s1 κ e2 s2 efs →
+  to_val e1 = None.
+Proof.
+  rewrite /prim_step.
+  move => [hes wes] [[ws vis] hprog] κ [hes' wes'] [[ws' vis'] hprog'] efs [HRed _].
+  inversion HRed => //=; subst.
+  destruct hes' => //.
+  eapply iris.val_head_stuck with (s1 := (hs, ws, [::], empty_instance)) (s2 := (hs', ws', [::], empty_instance)).
+  unfold iris.prim_step.
+  by repeat split => //.
+Qed.
+
+Lemma wasm_host_mixin : LanguageMixin of_val to_val prim_step.
+Proof. split; eauto using to_of_val, of_to_val, val_head_stuck. Qed.
+
+Canonical Structure wasm_host_lang := Language wasm_host_mixin.
+
+Implicit Type σ : state.
+
+(*
+Class wfuncG Σ := WFuncG {
+  func_invG :> invGS Σ;
+  func_gen_hsG :> gen_heapGS N function_closure Σ;
+}.
+
+Class wtabG Σ := WTabG {
+  tab_gen_hsG :> gen_heapGS (N*N) funcelem Σ;
+}.
+
+Class wmemG Σ := WMemG {
+  mem_gen_hsG :> gen_heapGS (N*N) byte Σ;
+}.
+
+Class wmemsizeG Σ := WMemsizeG {
+  memsize_gen_hsG :> gen_heapGS N N Σ;
+}.
+
+Class wglobG Σ := WGlobG {
+  glob_gen_hsG :> gen_heapGS N global Σ;
+}.
+
+Class wframeG Σ := WFrameG {
+  locs_gen_hsG :> ghost_mapG Σ unit frame;
+}.
+*)
+Require Export iris_wp_def.
+
+(* The host expands the memory model of Wasm by vi_store and a list of module declarations. *)
+
+Class hvisG Σ := HVisG {
+  vis_genG :> ghost_mapG Σ nat (list module_export)
+}.
+
+Class hmsG Σ := HMsG {
+  ms_genG :> ghost_mapG Σ N module
+}.
+
+
+
+Definition frameGName : positive := 10%positive.
+Definition visGName : positive := 11%positive.
+Definition msGName : positive := 12%positive.
+
+Definition proph_id := positive. (* ??? *)
+
+Instance eqdecision_frame: EqDecision frame.
+Proof. decidable_equality. Qed.
+
+Instance eqdecision_module: EqDecision module.
+Proof. move => m m'. unfold Decision. by decidable_equality. Qed.
+
+Global Instance host_heapG_irisG `{!wfuncG Σ, !wtabG Σ, !wmemG Σ, !wmemsizeG Σ, !wglobG Σ, !wframeG Σ, !hvisG Σ, !hmsG Σ} : weakestpre.irisGS wasm_host_lang Σ := {
+  iris_invGS := func_invG; (* ??? *)
+  state_interp σ _ κs _ :=
+    let: (s, vis, ms) := σ in
+     ((gen_heap_interp (gmap_of_list s.(s_funcs))) ∗
+      (gen_heap_interp (gmap_of_table s.(s_tables))) ∗
+      (gen_heap_interp (gmap_of_memory s.(s_mems))) ∗
+      (gen_heap_interp (gmap_of_list s.(s_globals))) ∗
+      (ghost_map_auth visGName 1 vis) ∗ 
+      (ghost_map_auth msGName 1 (gmap_of_list ms)) ∗
+      (* Should this really be here, though? *)
+      (ghost_map_auth frameGName 1 (<[ tt := empty_frame ]> ∅)) ∗ 
+      (gen_heap_interp (gmap_of_list (fmap mem_length s.(s_mems))))
+    )%I;
+    num_laters_per_step _ := 0;
+    fork_post _ := True%I;
+    state_interp_mono _ _ _ _ := fupd_intro _ _
+}.
+
+
+
+
+Section host_lifting.
+Context `{!wfuncG Σ, !wtabG Σ, !wmemG Σ, !wmemsizeG Σ, !wglobG Σ, !wframeG Σ, !hvisG Σ, !hmsG Σ}.
+
+
+(* adding this would nullify all lemmas in weakestpre -- why? Is this not the 
+   correct instance? *)
+(*
+Global Instance wp_host : Wp (iProp Σ) host_expr iris.val stuckness.
+Proof using Σ wfuncG0 wtabG0 wmemG0 wmemsizeG0 wglobG0 wframeG0 hvisG0 hmsG0.
+  by eapply weakestpre.wp'.
+Qed.
+*)
+
+Lemma wp_host_test_const (s: stuckness) E vs:
+  ⊢ wp s E (([::], (v_to_e_list vs)): host_expr) (λ v, ⌜ v = immV vs ⌝).
+Proof.
+  iApply weakestpre.wp_value => //.
+  unfold IntoVal => /=. by f_equal. 
+Qed.
+
+(*
+Let wp_wasm := @wp_wasm Σ wfuncG0.
+*)
+
+
+Definition reducible := @reducible wasm_host_lang.
+
+Let reduce := @reduce host_function host_instance.
+
+(* All the possible wasm expression that could appear in the host configuration, starting from empty *)
+Inductive host_wasm_expr_valid : list administrative_instruction -> Prop :=
+| HWEV_const: forall es,
+    const_list es ->
+    host_wasm_expr_valid es
+| HWEV_trap:
+    host_wasm_expr_valid [AI_trap]
+| HWEV_invoke: forall n,
+    host_wasm_expr_valid [AI_invoke n]
+| HWEV_local: forall n f es,
+    host_wasm_expr_valid [AI_local n f es].
+
+Hint Constructors host_wasm_expr_valid.
+
+(* Any possible wasm expression as defined above reduces independently from the frame. *)
+Lemma hwev_reduce_ignore_frame es hs ws f1 f2 hs' ws' f' es':
+  host_wasm_expr_valid es ->
+  reduce hs ws f1 es hs' ws' f' es' ->
+  reduce hs ws f2 es hs' ws' f2 es'.
+Proof.
+  move => Hhwev Hred.
+  inversion Hhwev; subst; clear Hhwev.
+  - by apply values_no_reduce in Hred.
+  - by apply test_no_reduce_trap in Hred.
+  - remember [AI_invoke n] as es0. induction Hred; subst => //=.
+    + inversion H; subst; clear H => //=; try by do 3 destruct vs => //.
+      move/lfilledP in H1.
+      inversion H1; subst; clear H1.
+      by do 2 destruct vs => //=.
+    + by eapply r_invoke_native => //=.
+    + move/lfilledP in H.
+      inversion H; subst; clear H => //; last by do 2 destruct vs => //.
+      destruct vs => //=.
+      2: { destruct vs, es, es'0 => //=. simpl in H1; inversion H1; subst; by simpl in H5. }
+      destruct es => /=; first by exfalso; eapply empty_no_reduce.
+      destruct es, es'0 => //=; simpl in H1.
+      inversion H1; subst; clear H1.
+      move/lfilledP in H0.
+      inversion H0; subst; clear H0.
+      simpl; rewrite cats0.
+      by apply IHHred.
+  - remember [AI_local n f es0] as es1. induction Hred => //=.
+    + inversion H; subst; clear H => //=; try by do 3 destruct vs => //.
+      * inversion H2; subst; clear H2.
+        by apply r_simple, rs_local_const.
+      * inversion H0; subst; clear H0.
+        by apply r_simple, rs_local_trap.
+      * inversion H3; subst; clear H3.
+        by apply r_simple; eapply rs_return.
+      * move/lfilledP in H1.
+        inversion H1; subst; clear H1.
+        by do 2 destruct vs => //=.
+    + by eapply r_invoke_native => //=.
+    + move/lfilledP in H.
+      inversion H; subst; clear H => //; last by do 2 destruct vs => //.
+      destruct vs => //=.
+      2: { destruct vs, es, es'0 => //=. simpl in H5; inversion H5; subst; by simpl in H1. }
+      destruct es => /=; first by exfalso; eapply empty_no_reduce.
+      destruct es, es'0 => //=; simpl in H5.
+      inversion H5; subst; clear H5.
+      move/lfilledP in H0.
+      inversion H0; subst; clear H0.
+      simpl; rewrite cats0.
+      by apply IHHred.
+    + by apply r_local.
+Qed.
+      
+(* The set of possible wasm expressions is closed wrt reduce. *)
+Lemma hwev_reduce_closed hs ws f es hs' ws' f' es':
+  host_wasm_expr_valid es ->
+  reduce hs ws f es hs' ws' f' es' ->
+  host_wasm_expr_valid es'.
+Proof.
+  move => Hhwev Hred.
+  inversion Hhwev; subst; clear Hhwev => /=.
+  - by apply values_no_reduce in Hred. 
+  - by apply test_no_reduce_trap in Hred.
+  - remember [AI_invoke n] as es0. induction Hred => //=.
+    + inversion H; subst; clear H => //=; try by do 3 destruct vs => //.
+    + move/lfilledP in H.
+      inversion H; subst; clear H => //; last by do 2 destruct vs => //.
+      destruct vs => //=.
+      2: { destruct vs, es, es'0 => //=. simpl in H5; inversion H5; subst; by simpl in H1. }
+      destruct es => /=; first by exfalso; eapply empty_no_reduce.
+      destruct es, es'0 => //=; simpl in H5.
+      inversion H5; subst; clear H5.
+      move/lfilledP in H0.
+      inversion H0; subst; clear H0.
+      simpl; rewrite cats0.
+      by apply IHHred.
+  - remember [AI_local n f0 es0] as es1.
+    induction Hred; subst => //=; try by do 3 destruct vcs => //=.
+    + inversion H; subst; clear H => //=; (try by do 3 destruct vs => //); by apply HWEV_const.
+    + move/lfilledP in H.
+      inversion H; subst; clear H => //; last by do 2 destruct vs => //.
+      destruct vs => //=.
+      2: { destruct vs, es, es'0 => //=. simpl in H1; inversion H1; subst; by simpl in H5. }
+      destruct es => /=; first by exfalso; eapply empty_no_reduce.
+      destruct es, es'0 => //=; simpl in H1.
+      inversion H1; subst; clear H1.
+      move/lfilledP in H0.
+      inversion H0; subst; clear H0.
+      simpl; rewrite cats0.
+      by apply IHHred.
+Qed.
+      
+(* Lifting reduction of valid wasm expressions to host configurations. *)
+Lemma reducible_lift es ws vis ms:
+  host_wasm_expr_valid es ->
+  iris_wp_def.reducible es (hs, ws, [], empty_instance) ->
+  reducible ([], es) (ws, vis, ms).
+Proof.
+  move => Hvalid.
+  unfold reducible, iris_wp_def.reducible, language.reducible, prim_step.
+  move => [κ [es' [σ' [efs HStep]]]].
+  destruct σ' as [[[hs' ws'] vs'] inst'].
+  exists [], ([], es'), (ws', vis, ms), [].
+  simpl in *.
+  destruct HStep as [HStep [-> ->]].
+  split => //.
+  eapply HR_wasm_step.
+  by eapply hwev_reduce_ignore_frame in Hvalid => //.
+Qed.
+
+(* Lifting wasm wp to host wp *)
+Lemma wp_host_wasm (s: stuckness) E (es: iris.expr) (Φ: iris.val -> iProp Σ):
+  (* wp_wasm s E es Φ *)
+  (* This abuse of notation is somehow possible. It is the weirdest thing I've 
+     seen in a while *)
+  host_wasm_expr_valid es ->
+  WP es @ s; E {{ Φ }}
+  ⊢ WP (([::], es): host_expr) @ s; E {{ Φ }}.
+Proof.
+  iLöb as "IH" forall (s E es Φ).
+  iIntros (Hhwev).
+  repeat rewrite weakestpre.wp_unfold /weakestpre.wp_pre /=.
+  repeat rewrite wp_unfold /wp_pre /=.
+  iIntros "Hwp".
+  destruct (iris.to_val es) eqn: Hes => //=.
+  iIntros ([[ws vis] ms] ns κ κs nt) "Hσ".
+  iSpecialize ("Hwp" $! (hs, ws, [::], empty_instance) ns κ κs nt).
+  iDestruct "Hσ" as "(Hwf & Hwt & Hwm & Hwg & Hvis & Hms & Hframe & Hmsize)".
+  iSpecialize ("Hwp" with "[$]").
+  iMod "Hwp" as "(%Hred & Hwp)".
+  iModIntro.
+  iSplit.
+  - destruct s => //.
+    iPureIntro.
+    by apply reducible_lift.
+  - iIntros ([hes' wes'] [[ws' vis'] ms'] efs HStep).
+    unfold Iris_host.prim_step in HStep.
+    destruct HStep as [HStep [-> ->]].
+    inversion HStep; subst; clear HStep.
+    iSpecialize ("Hwp" $! wes' (hs', ws', [::], empty_instance) [::] with "[%]"); first by unfold iris.prim_step.
+    iMod "Hwp".
+    do 2 iModIntro.
+    iMod "Hwp".
+    iModIntro.
+    iMod "Hwp".
+    iModIntro.
+    iDestruct "Hwp" as "((Hwf & Hwt & Hwm & Hwg & Hwframe & Hmsize) & Hwp)".
+    iDestruct "Hwp" as (f) "(Hf & Hwp & ?)".
+    iFrame.
+    iSplit => //.
+    iApply "IH"; first by apply hwev_reduce_closed in H0.
+    iApply "Hwp".
+    by iApply "Hf".
+Qed.
+  
+(*
+Section Host_wp_import.
+  (* Host wp must depend on the same memory model as for wasm *)
+  Context `{!wfuncG Σ, !wtabG Σ, !wmemG Σ, !wmemsizeG Σ, !wglobG Σ, !wframeG Σ}.
+
+  Record host_program_logic := {
+      wp_host (s : stuckness) : coPset -d> host_function -d> seq.seq value -d> (result -d> iPropO Σ) -d> iPropO Σ;
+      wp_host_not_stuck : (forall σ ns κs nt Φ h E vcs t1s t2s a, (let '(hs,s,_,_) := σ in
+                                              s_funcs s !! a = Some (FC_func_host (Tf t1s t2s) h)) ->
+                                              state_interp σ ns κs nt -∗
+                                              wp_host NotStuck E h vcs Φ ={E}=∗
+                                              state_interp σ ns κs nt ∗ wp_host NotStuck E h vcs Φ ∗
+                                              ⌜(let '(hs,s,_,_) := σ in (∃ hs' s' r, host_application hs s (Tf t1s t2s) h vcs hs' (Some (s',r))) ∨
+                                               (∃ hs', host_application hs s (Tf t1s t2s) h vcs hs' None))⌝);
+      wp_host_step_red : (∀ σ ns κ κs nt Φ h E vcs t1s t2s, (
+                                                               
+                                              state_interp σ ns (κ ++ κs) nt -∗
+                                              wp_host NotStuck E h vcs Φ ={E,∅}=∗
+                                              (∀ σ' r, ⌜(let '(hs,s,_,_) := σ in let '(hs',s',_,_) := σ' in host_application hs s (Tf t1s t2s) h vcs hs' (Some (s',r)))⌝
+                                              ={∅}▷=∗^(S $ num_laters_per_step ns) |={∅,E}=>
+                                                 state_interp σ' (S ns) κs nt ∗ Φ r) ∗
+                                              (∀ σ', ⌜(let '(hs,s,_,_) := σ in let '(hs',_,_,_) := σ' in host_application hs s (Tf t1s t2s) h vcs hs' None)⌝
+                                              ={∅}▷=∗^(S $ num_laters_per_step ns) |={∅,E}=>
+                                                 state_interp σ' (S ns) κs nt ∗ wp_host NotStuck E h vcs Φ)));
+    }.
+  
+End Host_wp_import.
+ *)
+
+  End host_lifting.
+
+
 End Iris_host.
